@prefix : <http://www.nebularis.org/ontologies/Mork/> .
@prefix owl: <http://www.w3.org/2002/07/owl#> .
@prefix rdf: <http://www.w3.org/1999/02/22-rdf-syntax-ns#> .
@prefix xml: <http://www.w3.org/XML/1998/namespace> .
@prefix xsd: <http://www.w3.org/2001/XMLSchema#> .
@prefix rdfs: <http://www.w3.org/2000/01/rdf-schema#> .
@base <http://www.nebularis.org/ontologies/Mork/> .

<http://www.nebularis.org/ontologies/Mork> rdf:type owl:Ontology ;
                                            owl:imports <http://www.w3.org/2004/02/skos/core> .

#################################################################
#    Annotation properties
#################################################################

###  http://purl.org/dc/terms/contributor
<http://purl.org/dc/terms/contributor> rdf:type owl:AnnotationProperty .


###  http://purl.org/dc/terms/creator
<http://purl.org/dc/terms/creator> rdf:type owl:AnnotationProperty .


###  http://purl.org/dc/terms/description
<http://purl.org/dc/terms/description> rdf:type owl:AnnotationProperty .


###  http://purl.org/dc/terms/title
<http://purl.org/dc/terms/title> rdf:type owl:AnnotationProperty .


###  http://www.nebularis.org/ontologies/Mork/userDeclined
:userDeclined rdf:type owl:AnnotationProperty ;
              rdfs:label "user declined" ;
              <http://www.w3.org/2004/02/skos/core#definition> "A note explaining that a user has declined the use of a DataMapping" ;
              rdfs:subPropertyOf <http://www.w3.org/2004/02/skos/core#note> .


#################################################################
#    Object Properties
#################################################################

###  http://www.nebularis.org/ontologies/Mork/associativeBroader
:associativeBroader rdf:type owl:ObjectProperty ;
                    rdfs:subPropertyOf <http://www.w3.org/2004/02/skos/core#broader> ;
                    owl:inverseOf :associativeNarrower ;
                    rdfs:label "associative broader" ;
                    <http://www.w3.org/2004/02/skos/core#definition> "extends skos:broader with the concept of associativity" ;
                    <http://www.w3.org/2004/02/skos/core#scopeNote> "By convention, associativeBroader is not used to make assertions. Rather, its subProperties should be used, however the superProperty exists in order to draw inferences about the transitive closure of a hierarchical relation." .


###  http://www.nebularis.org/ontologies/Mork/associativeNarrower
:associativeNarrower rdf:type owl:ObjectProperty ;
                     rdfs:subPropertyOf <http://www.w3.org/2004/02/skos/core#narrower> ;
                     rdfs:label "associative narrower" ;
                     <http://www.w3.org/2004/02/skos/core#definition> "extends skos:narrower with the concept of associativity" ;
                     <http://www.w3.org/2004/02/skos/core#scopeNote> "By convention, associativeNarrower is not used to make assertions. Rather, its subProperties should be used, however the superProperty exists in order to draw inferences about the transitive closure of a hierarchical relation." .


###  http://www.nebularis.org/ontologies/Mork/broadABoxCategoryMatch
:broadABoxCategoryMatch rdf:type owl:ObjectProperty ;
                        rdfs:subPropertyOf :broadCategoryMatch ;
                        owl:inverseOf :narrowABoxCategoryMatch ;
                        rdfs:label "has board a-box category match" ;
                        <http://www.w3.org/2004/02/skos/core#altLabel> "has a-box super-category match" ;
                        <http://www.w3.org/2004/02/skos/core#definition> """Used to state a mapping link where the subject maps to a broader category via object-property link to an individual that represents the Hyperonym (i.e., the more specific thing in the A-Box of the mapped concept scheme).

The A-Box (or Assertional Box) contains assertions (or facts) about individuals within the domain.""" ;
                        <http://www.w3.org/2004/02/skos/core#example> """###  http://www.example.org/Risks#isSubcategoryOf
:isSubcategoryOf rdf:type owl:ObjectProperty .

###  http://www.example.org/Risks#RegulatoryRisk
:RegulatoryRisk rdf:type owl:NamedIndividual ,
                                          risk:Risk .

###  http://www.example.org/Risks#PCIDSS
:PCIDSS rdf:type owl:NamedIndividual ,
            skos:note \"Hyperonymic relation via A-Box object property\" ;
            mork:hasMapping :PciDssMapping ;
            rdfs:comment \"we want to instantiate an axiom `:isSubcategoryOf :RegulatoryRisk' here\" .

###  http://www.example.org/Mapping#PciDssMapping
:PciDssMapping rdf:type owl:NamedIndividual ,
                      mork:DataMapping ;
            rdfs:comment \"the following statements assert the desired axiom for PCIDSS, viz `isSubcategoryOf :RegulatoryRisk'\" ;
            mork:exactTBoxMatch risk:Risk ;
            mork:exactRBoxMatch risk:isSubcategoryOf ;
            mork:broadABoxCategoryMatch risk:RegulatoryRisk .""" ;
                        <http://www.w3.org/2004/02/skos/core#scopeNote> """An ABox category match may apply either before or after a datum is to be individuated. In either case, the operation is implied to be idempotent.

An ABox category match implies the presence of both a RBox match (to the object property over which the relationship is to be defined) and a skos:mappingRelation to the owl:Individual in the A-box. This is not described in the domains for this property, since such constraints are better expressed as SWRL/SHACL constraints.""" .


###  http://www.nebularis.org/ontologies/Mork/broadCategoryMatch
:broadCategoryMatch rdf:type owl:ObjectProperty ;
                    rdfs:subPropertyOf <http://www.w3.org/2004/02/skos/core#broadMatch> ;
                    owl:inverseOf :narrowCategoryMatch ;
                    rdfs:label "has broad category match" ;
                    <http://www.w3.org/2004/02/skos/core#definition> "A broadCategoryMatch is used to state a hyperonymic, categorical mapping link between two conceptual resources in different concept schemes, where the subject is the (more specific) hyponym, and the object is the (more general) hyperonym." .


###  http://www.nebularis.org/ontologies/Mork/broadConceptRole
:broadConceptRole rdf:type owl:ObjectProperty ;
                  rdfs:subPropertyOf :associativeBroader ;
                  rdfs:range <http://www.w3.org/2004/02/skos/core#Concept> ;
                  rdfs:label "has objectified broad concept role" ;
                  rdfs:seeAlso :Objectification ;
                  <http://www.w3.org/2004/02/skos/core#definition> "Used to model the subject in an Objectification, i.e., a relationship between concepts that must be \"reified\" in order to annotate it, or create associations between the relationship and other concepts." ;
                  <http://www.w3.org/2004/02/skos/core#scopeNote> """This property is NOT marked as the inverse of narrowConceptRole, since doing so would cause the reasoner to assume that the participants in an Objectification are members of that class.

For situations where such extended reasoning is desireable, broadNavigableConceptRole and its inverse narrowNavigableConceptRole can be used.""" .


###  http://www.nebularis.org/ontologies/Mork/broadNavigableConceptRole
:broadNavigableConceptRole rdf:type owl:ObjectProperty ;
                           rdfs:subPropertyOf :broadConceptRole ;
                           owl:inverseOf :narrowNavigableConceptRole ;
                           rdfs:label "has navigable objectified broad concept role" ;
                           rdfs:seeAlso :Objectification ;
                           <http://www.w3.org/2004/02/skos/core#definition> "Extends broadConceptRole to model the subject in an Objectification where the participating concepts can be inferred to be members of the Objectification class" ;
                           <http://www.w3.org/2004/02/skos/core#scopeNote> """This property is the inverse of narrowNavigableConceptRole. The reasoner will assume Individuals related via this property are members of the class Objectification.

For situations where such reasoning is not desireable, use the superProperty broadConceptRole instead.""" .


###  http://www.nebularis.org/ontologies/Mork/broadRBoxCategoryMatch
:broadRBoxCategoryMatch rdf:type owl:ObjectProperty ;
                        rdfs:subPropertyOf :broadCategoryMatch ;
                        owl:inverseOf :narrowRBoxCategoryMatch ;
                        rdfs:label "has broad r-box category match" ;
                        rdfs:seeAlso :Objectification ;
                        <http://www.w3.org/2004/02/skos/core#definition> """Used to state a mapping link where the subject maps to a broader category of relationship (i.e., the more specific relation in the R-Box of the mapped concept scheme). This property is intended for use with members of the Objectification class, however no domain or range assertions are made in order to avoid having the reasoner incorrectly assign individuals to said class.

The R-Box (or Relational Box) defines the properties or roles that can be used to relate individuals, and thier characteristics, such as whether they are symmetric, transitive, or functional.""" ;
                        <http://www.w3.org/2004/02/skos/core#scopeNote> "Assertions made with this property are intended for use alongside matches to individuals in the A-Box of a target ontology." .


###  http://www.nebularis.org/ontologies/Mork/broadTBoxCategoryMatch
:broadTBoxCategoryMatch rdf:type owl:ObjectProperty ;
                        rdfs:subPropertyOf :broadCategoryMatch ;
                        owl:inverseOf :narrowTBoxCategoryMatch ;
                        rdfs:label "has broad t-box category match" ;
                        <http://www.w3.org/2004/02/skos/core#altLabel> "has t-box super-category match" ;
                        <http://www.w3.org/2004/02/skos/core#definition> """Used to define a hyperonymic, categorical relationship between concepts in different concept schemes, specifically modelling the subject as being in an owl:subclassOf relationship with the object.

The T-Box (or Terminological Box) defines the vocabulary of the domain by describing concepts (such as Classes) and roles (relationships that can be defined between objects).""" ;
                        <http://www.w3.org/2004/02/skos/core#scopeNote> "A TBox category must be applied before a datum can be individuated, since it implies the existence of an owl:Class not originally present in an OntologicalScheme. The implication here is that the operation resulting from this axiom is idempotent." .


###  http://www.nebularis.org/ontologies/Mork/broaderApplicative
:broaderApplicative rdf:type owl:ObjectProperty ;
                    rdfs:subPropertyOf :broaderMapping ;
                    rdf:type owl:AsymmetricProperty ;
                    rdfs:label "has broader applicative mapping" ;
                    <http://www.w3.org/2004/02/skos/core#definition> """Behaves like an applicative functor (i.e., a lax monoidal functor). This causes any compositeNarrowerMapping to be applied within the context (i.e., mapping outcome) of the object, rather than the subject.

Used when a mapping needs to interact with the outcome of a prior mapping, for example a compositeBroader or hypothesisMapping. Please read the skos:scopeNote for the expected behaviours.""" ;
                    <http://www.w3.org/2004/02/skos/core#scopeNote> """All compositeNarrowerMappings will be applied to the context (i.e., the axioms resulting as the *outcome* of the broaderApplicative object mapping). This implies the following rules:

- The broaderApplicative object must be a DataMapping or subclass thereof.
- An exactRBoxMatch or inverseRBoxMatch MUST be provided to indicate the relationship between the subject (outcome of this mapping) and the object (on the other end of the relationship).

Specifically, this instruction means:

- Consider the context/outcome axiom of this (subject) mapping, refer to it as the \"child\"
- Look up the broaderApplicative mapping, refer to it as the \"parent\"
- Find the axiom (or entry point into a digraph of axioms) created by the \"parent\" mapping, that is related to to the \"child\" axiom along the relationship defined by the exactRBoxMatch
- Apply the compositeNarrowerMappings of the subject (mapping) to the parent's axiom(s) and not to the child's""" .


###  http://www.nebularis.org/ontologies/Mork/broaderMapping
:broaderMapping rdf:type owl:ObjectProperty ;
                rdfs:subPropertyOf :relatedMapping ;
                owl:inverseOf :narrowerMapping ;
                rdfs:domain :DataMapping ,
                            [ owl:intersectionOf ( <http://www.w3.org/2004/02/skos/core#OrderedCollection>
                                                   [ rdf:type owl:Restriction ;
                                                     owl:onProperty <http://www.w3.org/2004/02/skos/core#member> ;
                                                     owl:someValuesFrom :DataMapping
                                                   ]
                                                 ) ;
                              rdf:type owl:Class
                            ] ;
                rdfs:range :DataMapping ;
                rdfs:label "has broader mapping" ;
                <http://www.w3.org/2004/02/skos/core#definition> "Relates a mapping to a mapping that is more general (less specific)" .


###  http://www.nebularis.org/ontologies/Mork/closeMapping
:closeMapping rdf:type owl:ObjectProperty ;
              rdfs:subPropertyOf :relatedMapping ;
              rdfs:label "has close mapping" ;
              <http://www.w3.org/2004/02/skos/core#definition> "used to link two mappings that are sufficiently similar that they can be used interchangeably in some applications." .


###  http://www.nebularis.org/ontologies/Mork/compositeBroader
:compositeBroader rdf:type owl:ObjectProperty ;
                  rdfs:subPropertyOf :associativeBroader ;
                  owl:inverseOf :compositeNarrower ;
                  rdfs:label "composite broader" ;
                  <http://www.w3.org/2004/02/skos/core#definition> "Extends associativeBroader with the concept of composition, wherein the object's existence is semantically conditional upon the subject's. This property is the inverse of compositeNarrower." .


###  http://www.nebularis.org/ontologies/Mork/compositeBroaderMapping
:compositeBroaderMapping rdf:type owl:ObjectProperty ;
                         rdfs:subPropertyOf :broaderMapping ;
                         owl:inverseOf :compositeNarrowerMapping ;
                         rdfs:label "has composite broader mapping" ;
                         rdfs:seeAlso :compositeNarrowerMapping ;
                         <http://www.w3.org/2004/02/skos/core#definition> "compositeBroaderMapping is used to compose mappings into a directed acyclic graph. The subject mapping is the component part of the object mapping. This is the inverse of compositeNarrowerMapping." ;
                         <http://www.w3.org/2004/02/skos/core#example> "See compositeNarrowerMapping for an example" .


###  http://www.nebularis.org/ontologies/Mork/compositeBroaderTemplate
:compositeBroaderTemplate rdf:type owl:ObjectProperty ;
                          rdfs:subPropertyOf :compositeBroaderMapping ;
                          owl:inverseOf :compositeNarrowerTemplate ;
                          rdfs:label "has composite broader template" ;
                          rdfs:seeAlso :templateMapping ;
                          <http://www.w3.org/2004/02/skos/core#definition> "Version of 'composite broader mapping' for use in templates. This property in the inverse of compositeNarrowerTemplate." .


###  http://www.nebularis.org/ontologies/Mork/compositeNarrower
:compositeNarrower rdf:type owl:ObjectProperty ;
                   rdfs:subPropertyOf :associativeNarrower ;
                   rdfs:label "composite narrower" ;
                   <http://www.w3.org/2004/02/skos/core#definition> "Extends associativeNarrower with the concept of composition, wherein the subject's existence is semantically conditional upon the object's. This property is the inverse of compositeBroader." .


###  http://www.nebularis.org/ontologies/Mork/compositeNarrowerMapping
:compositeNarrowerMapping rdf:type owl:ObjectProperty ;
                          rdfs:subPropertyOf :narrowerMapping ;
                          rdfs:comment "A concept in a TaxonomyScheme may well be broken down into multiple axioms when mapped to an OntologicalScheme. In this case, the digraph of mapping instructions can be constructed by relating mappings using this (and its inverse) property." ;
                          rdfs:label "has composite narrower mapping" ;
                          rdfs:seeAlso :compositeBroaderMapping ;
                          <http://www.w3.org/2004/02/skos/core#definition> "compositeNarrowerMapping is used to compose mappings into a directed acyclic graph. The object mapping is the component part of the subject mapping. This is the inverse of compositeBroaderMapping." ;
                          <http://www.w3.org/2004/02/skos/core#example> """Take some representation scheme, mapped from json: 

{
    \"aardvarkName\": \"Peter\",
    \"aardvarkSex\": \"M\"
}

This will yield two attributes, to which we will map three concepts in a concept scheme: aardvark, aardvark_Name, and aardvark_Sex.

In our ontology, we may wish to model aardvark within the t-box of the ontology:

:Aardvark rdf:type owl:Class;
            rdfs:subClassOf :Animal .

In this case, an input datum for aardvark will require that we define the class first, then assert a new individual which is a member of said class, before we can manage the input record by making DataTypeProperty assertions against the name and sex of the newly individuated animal.

Or indeed we might be required to model this by relating our new individual to some other fact within the a-box, adding meaning via object properties or annotations, e.g., using skos:

:Aardvark rdf:type owl:NamedIndividual ;
           <http://www.w3.org/2004/02/skos/core#narrowerTransitive> :Animal .

In either case, we are required to undertake multiple steps to individuate the record before we can begin to process the attributes that belong to (i.e. are narrower within) its concept scheme. This will yield a composition of mappings in order to create the necessary digraph in the target ontology scheme. The following example snippet (Turtle) positions the Aardvark concept in the T-Box of that target ontology, with subsequent individuals assigned to said class. Note the use of deferredMapping here, such that the class is composed of individuals, however the individuals cannot be asserted to belong to the class until it exists.

:MapAardvarkClass rdf:type owl:NamedIndividual ;
            rdfs:subClassOf mork:DataMapping ;
            mork:broadTBoxCategoryMatch ont:Animal ; 
            mork:compositeNarrowerMapping :MapAardvarkIndividual ;
            mork:conceptName \"Aardvark\" .

:MapAardvarkIndividual rdf:type owl:NamedIndividual ;
            rdfs:subClassOf mork:Datum ;
            mork:deferredMapping :MapAardvarkClass ;
            mork:compositeNarrowerMapping :MapAardvarkName, :MapAardvarkSex .

Subsequent mappings (for name and sex) may rely on these mappings as a hypothesis.""" .


###  http://www.nebularis.org/ontologies/Mork/compositeNarrowerTemplate
:compositeNarrowerTemplate rdf:type owl:ObjectProperty ;
                           rdfs:subPropertyOf :compositeNarrowerMapping ;
                           rdfs:label "has composite narrower template" ;
                           rdfs:seeAlso :templateMapping ;
                           <http://www.w3.org/2004/02/skos/core#definition> "Version of 'composite narrower mapping' for use in templates." .


###  http://www.nebularis.org/ontologies/Mork/concatenation
:concatenation rdf:type owl:ObjectProperty ;
               rdfs:subPropertyOf :placeholderMapping ;
               rdfs:label "concatenation" ;
               <http://www.w3.org/2004/02/skos/core#definition> "Used to indicate that a placeholderMapping is being used for the purposes of concatenating values" .


###  http://www.nebularis.org/ontologies/Mork/conceptScheme
:conceptScheme rdf:type owl:ObjectProperty ;
               rdfs:subPropertyOf <http://www.w3.org/2004/02/skos/core#inScheme> ;
               rdfs:range :TaxonomyScheme ;
               rdfs:label "in concept scheme" ;
               <http://www.w3.org/2004/02/skos/core#definition> "denotes the subject's membership in the object (TaxonomyScheme)" .


###  http://www.nebularis.org/ontologies/Mork/deferredMapping
:deferredMapping rdf:type owl:ObjectProperty ;
                 rdfs:subPropertyOf :relatedMapping ;
                 rdf:type owl:SymmetricProperty ;
                 rdfs:label "has deferred mapping" ;
                 <http://www.w3.org/2004/02/skos/core#definition> "Used to defer to a mapping where the subject is dependent on the result of applying the object (mapping) and obtaining the outcome. This can be used, for example, to ensure that individuals which belong to an owl:Class are processed only after the class axiom has been asserted." .


###  http://www.nebularis.org/ontologies/Mork/digraphMatch
:digraphMatch rdf:type owl:ObjectProperty ;
              rdfs:subPropertyOf <http://www.w3.org/2004/02/skos/core#broadMatch> ;
              owl:inverseOf :digraphOf ;
              rdfs:range :Digraph ;
              rdfs:label "has digraph match" ;
              owl:deprecated "Use compositeBroaderMapping and compositeNarrowerMapping instead." ;
              <http://www.w3.org/2004/02/skos/core#definition> "is used to state a hierarchical mapping link between conceptual resources in different concept schemes, where one concept is mapped to a directed (sub-)graph of related concepts." .


###  http://www.nebularis.org/ontologies/Mork/digraphOf
:digraphOf rdf:type owl:ObjectProperty ;
           rdfs:subPropertyOf <http://www.w3.org/2004/02/skos/core#narrowMatch> ;
           rdfs:domain :Digraph ;
           rdfs:label "is digraph match from" ;
           owl:deprecated "Use compositeBroaderMapping and compositeNarrowerMapping instead." ;
           <http://www.w3.org/2004/02/skos/core#definition> "digraphFrom is used to state a hierarchical mapping link between conceptual resources in different concept schemes, where concepts belong to a directed (sub-)graph that relates back to some parent concept (in another scheme)." .


###  http://www.nebularis.org/ontologies/Mork/elementType
:elementType rdf:type owl:ObjectProperty ;
             rdfs:subPropertyOf :compositeNarrower ;
             rdfs:domain :Collection ;
             rdfs:range :CollectionElement ;
             rdfs:label "element type" ;
             <http://www.w3.org/2004/02/skos/core#definition> "Specialises compositeNarrower with a particular semantics for describing the type of elements within a Collection. The domain and range for this property assertions provide an explicit hint to the reasoner as such." .


###  http://www.nebularis.org/ontologies/Mork/exactABoxMatch
:exactABoxMatch rdf:type owl:ObjectProperty ;
                rdfs:subPropertyOf :intransitiveExactMatch ;
                rdfs:label "exact A-Box match" ;
                <http://www.w3.org/2004/02/skos/core#definition> "Used to indicate an exact match to an element in the A-Box of an ontology (i.e., OntologicalScheme). The subject may come from any aspect of another domain (e.g., belonging to RepresentationScheme or TaxonomyScheme, coming from the T-Box, A-Box, or R-Box)." .


###  http://www.nebularis.org/ontologies/Mork/exactMapping
:exactMapping rdf:type owl:ObjectProperty ;
              rdfs:subPropertyOf :closeMapping ;
              rdfs:label "has exact mapping" ;
              <http://www.w3.org/2004/02/skos/core#definition> "used to link two mappings, indicating a high degree of confidence that they can be used interchangeably across a wide range of applications." .


###  http://www.nebularis.org/ontologies/Mork/exactRBoxMatch
:exactRBoxMatch rdf:type owl:ObjectProperty ;
                rdfs:subPropertyOf :intransitiveExactMatch ;
                rdfs:label "exact R-Box match" ;
                <http://www.w3.org/2004/02/skos/core#definition> "Used to indicate an exact match to an element in the R-Box of an ontology (i.e., OntologicalScheme). The subject may come from any aspect of another domain (e.g., belonging to RepresentationScheme or TaxonomyScheme, coming from the T-Box, A-Box, or R-Box)." .


###  http://www.nebularis.org/ontologies/Mork/exactTBoxMatch
:exactTBoxMatch rdf:type owl:ObjectProperty ;
                rdfs:subPropertyOf :intransitiveExactMatch ;
                rdfs:label "exact T-Box match" ;
                <http://www.w3.org/2004/02/skos/core#definition> """Used to indicate an exact match to an element in the T-Box of an ontology (i.e., OntologicalScheme). The subject may come from any aspect of another domain (e.g., belonging to RepresentationScheme or TaxonomyScheme, coming from the T-Box, A-Box, or R-Box).

The T-Box (or Terminological Box) defines the vocabulary of the domain by describing concepts (such as Classes) and roles (relationships that can be defined between objects).""" .


###  http://www.nebularis.org/ontologies/Mork/format
:format rdf:type owl:ObjectProperty ;
        rdfs:subPropertyOf owl:topObjectProperty ;
        rdfs:domain :RepresentationScheme ;
        rdfs:range :SerializationFormat ;
        rdfs:label "has format" ;
        <http://www.w3.org/2004/02/skos/core#definition> "denotes the SerializationFormat used by a RepresentationScheme" .


###  http://www.nebularis.org/ontologies/Mork/hasConcept
:hasConcept rdf:type owl:ObjectProperty ;
            rdfs:subPropertyOf owl:topObjectProperty ;
            owl:inverseOf <http://www.w3.org/2004/02/skos/core#inScheme> ;
            rdfs:label "has concept" ;
            <http://www.w3.org/2004/02/skos/core#altLabel> "contains concept" ;
            <http://www.w3.org/2004/02/skos/core#definition> "Denotes the membership of a skos:Concept in a skos:ConceptScheme. This property is the inverse of skos:inScheme" .


###  http://www.nebularis.org/ontologies/Mork/hasMapping
:hasMapping rdf:type owl:ObjectProperty ;
            rdfs:subPropertyOf <http://www.w3.org/2004/02/skos/core#relatedMatch> ;
            rdfs:domain [ rdf:type owl:Class ;
                          owl:unionOf ( [ rdf:type owl:Restriction ;
                                          owl:onProperty :conceptScheme ;
                                          owl:someValuesFrom :TaxonomyScheme
                                        ]
                                        [ rdf:type owl:Restriction ;
                                          owl:onProperty :representationScheme ;
                                          owl:someValuesFrom :RepresentationScheme
                                        ]
                                      )
                        ] ;
            rdfs:range [ rdf:type owl:Restriction ;
                         owl:onProperty :mappingScheme ;
                         owl:someValuesFrom :MappingScheme
                       ] ;
            rdfs:label "has mapping" ;
            <http://www.w3.org/2004/02/skos/core#definition> "Used to denote a mapping relation between a representation or concept scheme element and a mapping scheme element." ;
            <http://www.w3.org/2004/02/skos/core#scopeNote> "Whilst it is expected that concepts in a RepresentationScheme or TaxonomyScheme may directly leverage object properties in the skos:mappingRelation hierarchy, selection of a specific mapping may require intermediation via an individual in a MappingScheme. This property exists to support the latter construct." .


###  http://www.nebularis.org/ontologies/Mork/hypothesisMapping
:hypothesisMapping rdf:type owl:ObjectProperty ;
                   rdfs:subPropertyOf :relatedMapping ;
                   rdfs:label "has hypothesis mapping" ;
                   rdfs:seeAlso :compositeNarrowerMapping ;
                   <http://www.w3.org/2004/02/skos/core#definition> "used to provide a mapping (object) that is being used as a hypothesis in support of the (subject) mapping's postulated match" ;
                   <http://www.w3.org/2004/02/skos/core#example> """A hypothesis mapping can be used to support the weighting for another mapping. Borrowing the \"aardvark\" datum mapping example from the compositeNarrowerMapping skos:example, we can see the the concept mapping of aardvark_name may rely on the \"Aardvark Class\" mapping as a hypothesis, since if we have not mapped the axiom for the whole, then the part cannot be mapped either.

:Aardvark rdf:type owl:NamedIndividual ;
            rdfs:subClassOf mork:DataConcept ;
            mork:conceptScheme :Animals_Taxo ;
            skos:closeMatch :MapAardvarkClass ;
            mork::compositeNarrower :Aardvark_Name .

:Aardvark_Name rdf:type owl:NamedIndividual ;
            rdfs:subClassOf mork:DataConcept ;
            mork:conceptScheme :Animals_Taxo ;
            mork:compositeBroader :Aardvark ;
            skos:closeMatch :MapAardvark_Name .

:MapAardvark_Name rdf:type owl:NamedIndividual ;
            rdfs:subClassOf mork:DataMapping ;
            mork:hypothesisMapping :MapAardvarkClass ;
            skos:closeMatch :Ont_prop_Animal_Name .

:MapAardvarkClass rdf:type owl:NamedIndividual ;
            rdfs:subClassOf mork:DataMapping ;
            mork:broadClassMatch ont:Animal ;
            mork:compositeNarrowerMapping :MapAardvarkIndividual ;
            mork:conceptName \"Aardvark\" .

:MapAardvarkIndividual rdf:type owl:NamedIndividual ;
            rdfs:subClassOf datarep:Datum ;
            mork:deferredMapping :MapAardvarkClass .

This is a somewhat unnecessary hypothesis, since it is assumed that a processing logic would traverse the concept scheme for the taxa and fail the parent (aardvark) mapping before arriving at its component properties, however it provides an illustration of the use of this construct.""" .


###  http://www.nebularis.org/ontologies/Mork#identityTemplateMapping
:identityTemplateMapping rdf:type owl:ObjectProperty ;
                         rdfs:subPropertyOf :templateMapping ;
                         <http://www.w3.org/2004/02/skos/core#definition> "Used to indicate a deferredMapping (which this is a sub-object-property of) between the subject and some object(s) upon which individual of the subject is dependent. Unlike deferredMapping, this property is not symmetric." ;
                         <http://www.w3.org/2004/02/skos/core#example> "Aardvark is identified by its 'name' property, and thus we must process the 'name' mapping first and use the outcome of this mapping to determine the correct IRI/identity for each individual aardvark we come across." .


###  http://www.nebularis.org/ontologies/Mork#intransitiveExactMatch
:indicativeMapping rdf:type owl:ObjectProperty ;
                   rdfs:subPropertyOf :hasMapping ;
                   rdfs:label "indicative mapping" ;
                   <http://www.w3.org/2004/02/skos/core#definition> "Used to denote a potential mapping relation between a representation or concept scheme element and a mapping scheme element, suggesting that the subject may be an indicator for the existence of the object." .


###  http://www.nebularis.org/ontologies/Mork/interpolationComponent
:interpolationComponent rdf:type owl:ObjectProperty ;
                        rdfs:subPropertyOf <http://www.w3.org/2004/02/skos/core#member> ;
                        rdfs:domain <http://www.w3.org/2004/02/skos/core#OrderedCollection> ;
                        rdfs:range [ rdf:type owl:Class ;
                                     owl:unionOf ( [ owl:intersectionOf ( :DataMapping
                                                                          [ rdf:type owl:Restriction ;
                                                                            owl:onProperty :dataRef ;
                                                                            owl:someValuesFrom xsd:string
                                                                          ]
                                                                        ) ;
                                                     rdf:type owl:Class
                                                   ]
                                                   [ rdf:type owl:Restriction ;
                                                     owl:onProperty :dataInline ;
                                                     owl:minCardinality "1"^^xsd:nonNegativeInteger
                                                   ]
                                                 )
                                   ] ;
                        rdfs:label "has template component (member)" ;
                        rdfs:seeAlso :Interpolation ;
                        <http://www.w3.org/2004/02/skos/core#definition> "Relates an InterpolationTemplate to one of its members." .


###  http://www.nebularis.org/ontologies/Mork/intransitiveExactMatch
:intransitiveExactMatch rdf:type owl:ObjectProperty ;
                        rdfs:subPropertyOf <http://www.w3.org/2004/02/skos/core#closeMatch> ;
                        rdf:type owl:SymmetricProperty ;
                        rdfs:label "has (intransitive) exact match" ;
                        <http://www.w3.org/2004/02/skos/core#definition> "This is an intransitive version of skos:exactMatch. It is used to indicate what we believe to be a semantically exact match between concepts in different concept schemes." .


###  http://www.nebularis.org/ontologies/Mork#inverseRBoxMatch
:inverseRBoxMatch rdf:type owl:ObjectProperty ;
                  rdfs:subPropertyOf :exactRBoxMatch ;
                  rdfs:label "exact inverse R-Box match" ;
                  <http://www.w3.org/2004/02/skos/core#definition> """Used to indicate an exact match to the inverse of an element in the R-Box of an ontology (i.e., OntologicalScheme). 

This is required for situations where the inverse of a datatype or object property must be referenced but no explicit axiom exists for the binding.

The subject may come from any aspect of another domain (e.g., belonging to RepresentationScheme or TaxonomyScheme, coming from the T-Box, A-Box, or R-Box).""" ;
                  <http://www.w3.org/2004/02/skos/core#scopeNote> "NB: This property is NOT the inverse of exactRBoxMatch, but rather it represents the same semantics when referencing the inverse of the property." .


###  http://www.nebularis.org/ontologies/Mork#mappingScheme
:mappingScheme rdf:type owl:ObjectProperty ;
               rdfs:subPropertyOf <http://www.w3.org/2004/02/skos/core#inScheme> ;
               rdfs:range :MappingScheme ;
               rdfs:label "in mapping scheme" ;
               <http://www.w3.org/2004/02/skos/core#definition> "denotes the subject's membership in the object MappingScheme" .


###  http://www.nebularis.org/ontologies/Mork#memberOf
:memberOf rdf:type owl:ObjectProperty ;
          rdfs:subPropertyOf :compositeBroader ;
          owl:inverseOf :memberProperty ;
          rdfs:label "member property of" ;
          rdfs:seeAlso :memberProperty ;
          <http://www.w3.org/2004/02/skos/core#definition> "Defines the object as a component property (i.e., member) of the subject, primarily to describe Representation elements using a clear vocabulary. This property is the inverse of memberProperty." .


###  http://www.nebularis.org/ontologies/Mork#memberProperty
:memberProperty rdf:type owl:ObjectProperty ;
                rdfs:subPropertyOf :compositeNarrower ;
                rdf:type owl:AsymmetricProperty ,
                         owl:IrreflexiveProperty ;
                rdfs:label "member property" ;
                <http://www.w3.org/2004/02/skos/core#definition> """Defines the subject as a component property (i.e., member) of the object. This specialisation of compositeNarrower provides a clear vocabulary for describing member properties (i.e., associations via property) within Representation schemes.

Note that memberProperty is both asymmetric and irreflexive.""" ;
                <http://www.w3.org/2004/02/skos/core#example> """###  http://www.nebularis.org/hyperthunk/Mapping#Rep_Issuer
:Rep_Issuer rdf:type owl:NamedIndividual ,
                     mork:DataConcept ,
                     mork:Entity ;
            mork:conceptScheme :Mapping_Taxa ;
            mork:memberProperty :Rep_IssuerID ;
            mork:representationOf :Rep_Issuer ;
            mork:representationScheme :Mapping_Representation ;
            mork:identifier \"issuer\" ;
            skos:note \"Individual Representation Rep_Issuer\" .""" .


###  http://www.nebularis.org/ontologies/Mork#missingOrUnrelatedMatch
:missingOrUnrelatedMatch rdf:type owl:ObjectProperty ;
                         rdfs:subPropertyOf <http://www.w3.org/2004/02/skos/core#relatedMatch> ;
                         rdfs:label "missing or unrelated match" ;
                         owl:deprecated "Do not use" .


###  http://www.nebularis.org/ontologies/Mork#narrowABoxCategoryMatch
:narrowABoxCategoryMatch rdf:type owl:ObjectProperty ;
                         rdfs:subPropertyOf :narrowCategoryMatch ;
                         rdfs:label "has narrow a-box category match" ;
                         <http://www.w3.org/2004/02/skos/core#altLabel> "has a-box sub-category match" ;
                         <http://www.w3.org/2004/02/skos/core#definition> """Used to state a mapping link where the subject maps to a narrower category via object-property link to an individual that represents the Hyperonym (i.e., the more specific thing in the A-Box of the mapped concept scheme).

The A-Box (or Assertional Box) contains assertions (or facts) about individuals within the domain.""" ;
                         <http://www.w3.org/2004/02/skos/core#scopeNote> """An ABox category match may apply either before or after a datum is to be individuated. In either case, the operation is implied to be idempotent.

An ABox category match implies the presence of both a TBox match (to the object property over which the relationship is to be defined) and a skos:mappingRelation to the owl:Individual in the a-box, as described in the domains for this property.""" .


###  http://www.nebularis.org/ontologies/Mork#narrowCategoryMatch
:narrowCategoryMatch rdf:type owl:ObjectProperty ;
                     rdfs:subPropertyOf <http://www.w3.org/2004/02/skos/core#narrowMatch> ;
                     rdfs:label "has narrow category match" ;
                     <http://www.w3.org/2004/02/skos/core#definition> "A narrowCategoryMatch is used to state a hyperonymic, categorical mapping link between two conceptual resources in different concept schemes, where the subject is the (more general) hyperonym and the object is the (more specific) hyponym." .


###  http://www.nebularis.org/ontologies/Mork#narrowConceptRole
:narrowConceptRole rdf:type owl:ObjectProperty ;
                   rdfs:subPropertyOf :associativeNarrower ;
                   rdfs:range <http://www.w3.org/2004/02/skos/core#Concept> ;
                   rdfs:label "has objectified narrow concept role" ;
                   <http://www.w3.org/2004/02/skos/core#definition> "Used to model the object in association Objectification, i.e., a relationship between concepts that must be \"reified\" in order to annotate it, or create associations between the relationship and other concepts." .


###  http://www.nebularis.org/ontologies/Mork#narrowNavigableConceptRole
:narrowNavigableConceptRole rdf:type owl:ObjectProperty ;
                            rdfs:subPropertyOf :narrowConceptRole ;
                            rdfs:label "has navigable objectified narrow concept role" ;
                            rdfs:seeAlso :Objectification ;
                            <http://www.w3.org/2004/02/skos/core#definition> "Extends narrowConceptRole to model the object in an Objectification where the participating concepts can be inferred to be members of the Objectification class" ;
                            <http://www.w3.org/2004/02/skos/core#scopeNote> """This property is the inverse of broadNavigableConceptRole. The reasoner will assume Individuals related via this property are members of the class Objectification.

For situations where such reasoning is not desireable, use the superProperty narrowConceptRole instead.""" .


###  http://www.nebularis.org/ontologies/Mork#narrowRBoxCategoryMatch
:narrowRBoxCategoryMatch rdf:type owl:ObjectProperty ;
                         rdfs:subPropertyOf :narrowCategoryMatch ;
                         rdfs:label "has narrow r-box category match" ;
                         rdfs:seeAlso :Objectification ;
                         <http://www.w3.org/2004/02/skos/core#definition> """Used to state a mapping link where the subject maps to a narrower category of relationship (i.e., the more general relation in the R-Box of the mapped concept scheme). This property is intended for use with members of the Objectification class, however no domain or range assertions are made in order to avoid having the reasoner incorrectly assign individuals to said class.

The R-Box (or Relational Box) defines the properties or roles that can be used to relate individuals, and thier characteristics, such as whether they are symmetric, transitive, or functional.""" .


###  http://www.nebularis.org/ontologies/Mork#narrowTBoxCategoryMatch
:narrowTBoxCategoryMatch rdf:type owl:ObjectProperty ;
                         rdfs:subPropertyOf :narrowCategoryMatch ;
                         rdfs:label "has narrow t-box match" ;
                         <http://www.w3.org/2004/02/skos/core#altLabel> "has t-box sub-category match" ;
                         <http://www.w3.org/2004/02/skos/core#definition> """Used to define a hyperonymic, categorical relationship between concepts in different concept schemes, specifically modelling the subject as being the superclass in an owl:subclassOf relationship with the object.

The T-Box (or Terminological Box) defines the vocabulary of the domain by describing concepts (such as Classes) and roles (relationships that can be defined between objects).""" ;
                         <http://www.w3.org/2004/02/skos/core#scopeNote> "A TBox category must be applied before a datum can be individuated, since it implies the existence of an owl:Class not originally present in an OntologicalScheme. The implication here is that the operation resulting from this axiom is idempotent." .


###  http://www.nebularis.org/ontologies/Mork#narrowerMapping
:narrowerMapping rdf:type owl:ObjectProperty ;
                 rdfs:subPropertyOf :relatedMapping ;
                 rdfs:domain :DataMapping ;
                 rdfs:range :DataMapping ,
                            [ owl:intersectionOf ( <http://www.w3.org/2004/02/skos/core#OrderedCollection>
                                                   [ rdf:type owl:Restriction ;
                                                     owl:onProperty <http://www.w3.org/2004/02/skos/core#member> ;
                                                     owl:someValuesFrom :DataConcept
                                                   ]
                                                 ) ;
                              rdf:type owl:Class
                            ] ;
                 rdfs:label "has narrower mapping" ;
                 <http://www.w3.org/2004/02/skos/core#definition> "Relates a mapping to a mapping that is more specific" .


###  http://www.nebularis.org/ontologies/Mork#ontologicalScheme
:ontologicalScheme rdf:type owl:ObjectProperty ;
                   rdfs:subPropertyOf <http://www.w3.org/2004/02/skos/core#inScheme> ;
                   rdfs:range :OntologicalScheme ;
                   rdfs:label "in ontological scheme" ;
                   <http://www.w3.org/2004/02/skos/core#definition> "Denotes the subject membership in an OntologicalScheme. Note that this is designed for use only by inference based on SWRL or SHACL constraints, and should not be used directly (since there is no hint on the Domain)" .


###  http://www.nebularis.org/ontologies/Mork#referenceDataMapping
:placeholderMapping rdf:type owl:ObjectProperty ;
                    rdfs:subPropertyOf owl:topObjectProperty ;
                    rdfs:domain :DataMapping ;
                    rdfs:range [ owl:intersectionOf ( :Interpolation
                                                      [ rdf:type owl:Restriction ;
                                                        owl:onProperty :interpolationComponent ;
                                                        owl:someValuesFrom [ rdf:type owl:Class ;
                                                                             owl:unionOf ( [ rdf:type owl:Restriction ;
                                                                                             owl:onProperty :dataRef ;
                                                                                             owl:someValuesFrom xsd:string
                                                                                           ]
                                                                                           [ rdf:type owl:Restriction ;
                                                                                             owl:onProperty :dataInline ;
                                                                                             owl:minCardinality "1"^^xsd:nonNegativeInteger
                                                                                           ]
                                                                                         )
                                                                           ]
                                                      ]
                                                    ) ;
                                 rdf:type owl:Class
                               ] ;
                    rdfs:label "has placeholder mapping" ;
                    <http://www.w3.org/2004/02/skos/core#definition> "Indicates that a mapping defers to a collection of \"placeholders\" for values that should be derived at processing time" .


###  http://www.nebularis.org/ontologies/Mork/referenceDataMapping
:referenceDataMapping rdf:type owl:ObjectProperty ;
                      rdfs:subPropertyOf :templateMapping ;
                      rdfs:range [ rdf:type owl:Restriction ;
                                   owl:onProperty :dataRef ;
                                   owl:someValuesFrom xsd:string
                                 ] ;
                      rdfs:label "has reference data mapping" ;
                      rdfs:seeAlso :Lookup ;
                      <http://www.w3.org/2004/02/skos/core#definition> "Used to denote that a mapping takes a value from some input data (via dataRef), and matches it to a subject which contains an exact match on either the contents of its dataInline or the name of the individual." ;
                      <http://www.w3.org/2004/02/skos/core#example> """:Mapping_Contract_LOB rdf:type owl:NamedIndividual , mork:Datum ;
    mork:mappingScheme :Example_Scheme ;
    mork:exactTBoxMatch :Contract ;
    mork:referenceDataMapping :Mapping_Lob ;
    mork:compositeNarrowerMapping :Mapping_Contract_Details .

[ rdf:type owl:Axiom ;
  owl:annotatedSource :Mapping_Contract_LOB ;
  owl:annotationProperty mork:referenceDataMapping ;
  owl:annotatedTarget :Mapping_Lob ;
  skos:note \"lob may be determined by a lookup on the value contained in the lineOfBusiness field\" ] .

:Mapping_Lob rdf:type owl:NamedIndividual , mork:Lookup ;
    mork:mappingScheme :Example_Scheme ;
    mork:exactRBoxMatch :lob ;
    mork:exactTBoxMatch :LineOfBusiness ;
    mork:dataRef \"path.to.data.field.lineOfBusiness\" ;
    skos:note \"Line of business code maps to 'lob LineOfBusiness', via reference data lookup\" .""" ;
                      <http://www.w3.org/2004/02/skos/core#scopeNote> "If the name of the individual is to be used, then the value of the object's dataInline MUST be set to \"\"." .


###  http://www.nebularis.org/ontologies/Mork#relatedMapping
:relatedMapping rdf:type owl:ObjectProperty ;
                rdfs:subPropertyOf <http://www.w3.org/2004/02/skos/core#related> ;
                rdfs:comment "These concept mapping relations mirror mapping relations, and the data model defined below is similar. A distinct vocabulary is provided for describing the semantic and structural relationships between mappings, to provide a convenient way to differentiate links within a mapping scheme from links between different schemes." ;
                rdfs:label "has related mapping" ;
                <http://www.w3.org/2004/02/skos/core#definition> "used to describe a relationships between two potential mappings" .


###  http://www.nebularis.org/ontologies/Mork#representationOf
:representationOf rdf:type owl:ObjectProperty ;
                  rdfs:subPropertyOf <http://www.w3.org/2004/02/skos/core#relatedMatch> ;
                  owl:inverseOf :representedAs ;
                  rdfs:label "is representation of" ;
                  rdfs:seeAlso :DataConcept ,
                               :Representation ;
                  <http://www.w3.org/2004/02/skos/core#definition> "Used to indicate that a Representation can be used for a given DataConcept. NB: it is perfectly reasonable for an individual to belong to both the Representation and DataConcept classes, therefore this property can be used by an individual to refer to itself." .


###  http://www.nebularis.org/ontologies/Mork#representationScheme
:representationScheme rdf:type owl:ObjectProperty ;
                      rdfs:subPropertyOf <http://www.w3.org/2004/02/skos/core#inScheme> ;
                      rdfs:range :RepresentationScheme ;
                      rdfs:label "in representation scheme" ;
                      <http://www.w3.org/2004/02/skos/core#definition> "Denotes the subject's membership in the object RepresentationScheme" .


###  http://www.nebularis.org/ontologies/Mork#representedAs
:representedAs rdf:type owl:ObjectProperty ;
               rdfs:subPropertyOf <http://www.w3.org/2004/02/skos/core#relatedMatch> ;
               rdfs:label "is represented as" ;
               <http://www.w3.org/2004/02/skos/core#definition> "Used to describe one of the (potentially multiple) Representations of a DataConcept. This property is the inverse of representationOf." .


###  http://www.nebularis.org/ontologies/Mork#templateMapping
:templateMapping rdf:type owl:ObjectProperty ;
                 rdfs:subPropertyOf :deferredMapping ;
                 rdfs:label "has template mapping" ;
                 <http://www.w3.org/2004/02/skos/core#definition> """Used to denote a deferred mapping where the subject and the object together provide partial mapping semantics and must therefore be taken as a whole by a processing engine.

This mechanism can be used to reduce the number of assertions required in order to fulfil a mapping, since the object can act as a template - providing partial mapping semantics - and leave the specific details of the mapping to the subject.""" ;
                 <http://www.w3.org/2004/02/skos/core#scopeNote> """When a partial mapping intended for use as a \"template\" is created, any compositeNarrowerMapping that is also a partial (rather than a complete) mapping, should be associated via compositeNarrowerTemplate.

NB: where multiple composite narrower mappings exist on both the subject and object, the following semantics shall apply:

If the narrower mapping on the subject explicitly refers to a narrower mapping of the object, that assertion shall take precidence. 

If the composite narrower mappings of both the subject and the object are modelled using skos:OrderedCollection, then the ordering of both collections will be respected. Should the size of the respective collections differ, the smaller of the two will be taken as the range of applicable mappings for the whole.

If the composite narrower mappings of either subject or object are members of the DataMapping class or subclasses thereof and, members (by inference) of the IndexedMapping class, then the mappingIndex shall be used to correlate the templates and non-templates together, whether via exact indexA == indexB semantics, or by linking the indexes to the ordering of an skos:OrderedCollection.""" .


###  http://www.nebularis.org/ontologies/Mork#weightedBroader
:weightedBroader rdf:type owl:ObjectProperty ;
                 rdfs:subPropertyOf :broaderMapping ;
                 owl:inverseOf :weightedNarrower ;
                 rdfs:label "has weighted broader" ;
                 <http://www.w3.org/2004/02/skos/core#definition> "used to indicate that the subject has a lower weighting (and thereby is a broader match), compared to the object - this property is the inverse of weightedNarrower" .


###  http://www.nebularis.org/ontologies/Mork#weightedNarrower
:weightedNarrower rdf:type owl:ObjectProperty ;
                  rdfs:subPropertyOf :narrowerMapping ;
                  rdfs:label "has weighted narrower" ;
                  <http://www.w3.org/2004/02/skos/core#definition> "Used to indicate that the object has a higher weighting (and thereby is a narrower match), compared to the subject. Explicitly means that the object is a more likely match than the subject." .


#################################################################
#    Data properties
#################################################################

###  http://www.nebularis.org/ontologies/Mork#collectionElementScalarValue
:collectionElementScalarValue rdf:type owl:DatatypeProperty ;
                              rdfs:subPropertyOf owl:topDataProperty ;
                              <http://www.w3.org/2004/02/skos/core#scopeNote> """Not for external use. This datatype property is used as a placeholder super-property for generated owl:DataTypeProperty axioms which are used to hold the rdfs/xsd range for individuals in the Attribute and ScalarValueElement classes.

This specific property is exclusively used to manage Objectification.""" .


###  http://www.nebularis.org/ontologies/Mork#conceptFQNameTemplate
:conceptFQNameTemplate rdf:type owl:DatatypeProperty ;
                       rdfs:subPropertyOf :conceptNameTemplate .


###  http://www.nebularis.org/ontologies/Mork#conceptId
:conceptId rdf:type owl:DatatypeProperty ;
           rdfs:subPropertyOf :identifier ,
                              <http://www.w3.org/2004/02/skos/core#notation> ;
           rdf:type owl:FunctionalProperty ;
           rdfs:domain <http://www.w3.org/2004/02/skos/core#Concept> ;
           rdfs:range xsd:string ;
           rdfs:label "concept id" ;
           <http://www.w3.org/2004/02/skos/core#definition> "Specialises identifier for use in denoting the id of a DataConcept" .


###  http://www.nebularis.org/ontologies/Mork#conceptName
:conceptName rdf:type owl:DatatypeProperty ;
             rdfs:subPropertyOf :name .


###  http://www.nebularis.org/ontologies/Mork#conceptNameTemplate
:conceptNameTemplate rdf:type owl:DatatypeProperty ;
                     rdfs:subPropertyOf :template ;
                     <http://www.w3.org/2004/02/skos/core#definition> "Template for a concept name" ;
                     <http://www.w3.org/2004/02/skos/core#example> ":Subject mork:conceptNameTemplate \"Item{$name}\"" .


###  http://www.nebularis.org/ontologies/Mork#conceptShortNameTemplate
:conceptShortNameTemplate rdf:type owl:DatatypeProperty ;
                          rdfs:subPropertyOf :conceptNameTemplate .


###  http://www.nebularis.org/ontologies/Mork#data
:data rdf:type owl:DatatypeProperty ;
      rdfs:subPropertyOf owl:topDataProperty .


###  http://www.nebularis.org/ontologies/Mork#dataInline
:dataInline rdf:type owl:DatatypeProperty ;
            rdfs:subPropertyOf :data .


###  http://www.nebularis.org/ontologies/Mork#dataRef
:dataRef rdf:type owl:DatatypeProperty ;
         rdfs:subPropertyOf :data .


###  http://www.nebularis.org/ontologies/Mork#externalPropertyValue
:externalPropertyValue rdf:type owl:DatatypeProperty ;
                       rdfs:subPropertyOf owl:topDataProperty ;
                       <http://www.w3.org/2004/02/skos/core#scopeNote> "Not for external use. This datatype property is used as a placeholder super-property for generated owl:DataTypeProperty axioms which are used to hold the rdfs/xsd range for individuals in the Attribute class." .


###  http://www.nebularis.org/ontologies/Mork#identifier
:identifier rdf:type owl:DatatypeProperty ;
            rdfs:subPropertyOf owl:topDataProperty ;
            rdfs:label "identifier" ;
            <http://www.w3.org/2004/02/skos/core#definition> "Is used to mark a Representation or DataConcept with an identifier used by some external scheme or schema." ;
            <http://www.w3.org/2004/02/skos/core#note> """###  In this example, the 'identifier' denotes the JSON element/property name,
###  whilst the 'path' denotes the location in the json document.
###

:JS_Array_ContractingParties rdf:type owl:NamedIndividual, mork:Array ;
                   mork:elementType :JS_Elem_ContractingParties ;
                   mork:identifier \"contractingParties\" ;
                   mork:path \"contract.signatories.contractingParties\" .""" .


###  http://www.nebularis.org/ontologies/Mork/incompleteMapping
:incompleteMapping rdf:type owl:DatatypeProperty ;
                   rdfs:subPropertyOf owl:topDataProperty ;
                   rdfs:range xsd:boolean .


###  http://www.nebularis.org/ontologies/Mork/interpolationTemplate
:interpolationTemplate rdf:type owl:DatatypeProperty ;
                       rdfs:subPropertyOf :template ;
                       rdfs:range xsd:string ;
                       rdfs:seeAlso :Interpolation ;
                       <http://www.w3.org/2004/02/skos/core#definition> "Used to indicate a runtime interpolation of dataRef and/or dataInline values into a new string." ;
                       <http://www.w3.org/2004/02/skos/core#example> """:SomeMapping rdf:type owl:NamedIndividual , mork:Datum ;
    mork:dataRef \"path.to.processing-context.data.id\" ;
    mork:dataInline \"ID\" ;
    mork:interpolationTemplate \"The ${mork:dataInline} is: ${mork:dataRef}\" .""" ;
                       <http://www.w3.org/2004/02/skos/core#scopeNote> """Allows the values assigned to datatype properties to be referenced for string interpolation. Referenced properties are evaluated against properties relating to the subject of the assertion.

This datatype property can be used in one of two ways:

1. to combine datatype properties from the assertion context with string literals/interpolation - see the skos:example on the Interpolation class for details.

2. to provide a template for interpolating placeholder data into a new value, see the skos:example on this property for details..""" .


###  http://www.nebularis.org/ontologies/Mork/iri
:iri rdf:type owl:DatatypeProperty ;
     rdfs:subPropertyOf :conceptId ;
     rdf:type owl:FunctionalProperty ;
     rdfs:domain :OwlAxiom ;
     rdfs:label "identifier iri" ;
     <http://www.w3.org/2004/02/skos/core#definition> "Is used to identify a skos:Concept via a fully qualified IRI" .


###  http://www.nebularis.org/ontologies/Mork#itemsConstrained
:itemsConstrained rdf:type owl:DatatypeProperty ;
                  rdfs:subPropertyOf owl:topDataProperty ;
                  rdfs:range xsd:boolean .


###  http://www.nebularis.org/ontologies/Mork#mappingIndex
:mappingIndex rdf:type owl:DatatypeProperty ;
              rdfs:subPropertyOf owl:topDataProperty ;
              rdfs:label "mapping index" ;
              <http://www.w3.org/2004/02/skos/core#definition> "used to denote the index of a mapping where it occurs within a collection of mappings." .


###  http://www.nebularis.org/ontologies/Mork#name
:name rdf:type owl:DatatypeProperty ;
      rdfs:subPropertyOf owl:topDataProperty ;
      rdfs:range xsd:string ;
      <http://www.w3.org/2004/02/skos/core#definition> "composes" .


###  http://www.nebularis.org/ontologies/Mork#orderedItems
:orderedItems rdf:type owl:DatatypeProperty ;
              rdfs:subPropertyOf :itemsConstrained .


###  http://www.nebularis.org/ontologies/Mork#path
:path rdf:type owl:DatatypeProperty ;
      rdfs:subPropertyOf :identifier ;
      rdfs:label "has path" ;
      <http://www.w3.org/2004/02/skos/core#definition> "Is used to denote a \"path expression\" that locates a Representation within an externally defined scheme or schema." .


###  http://www.nebularis.org/ontologies/Mork#reference
:reference rdf:type owl:DatatypeProperty ;
           rdfs:subPropertyOf :identifier .


###  http://www.nebularis.org/ontologies/Mork#template
:template rdf:type owl:DatatypeProperty ;
          rdfs:subPropertyOf owl:topDataProperty ;
          <http://www.w3.org/2004/02/skos/core#definition> "used to store templates for the generation of identifiers within a merged graph" .


###  http://www.nebularis.org/ontologies/Mork#uniqueItems
:uniqueItems rdf:type owl:DatatypeProperty ;
             rdfs:subPropertyOf :itemsConstrained .


###  http://www.nebularis.org/ontologies/Mork#weighting
:weighting rdf:type owl:DatatypeProperty ;
           rdfs:subPropertyOf owl:topDataProperty ;
           rdfs:range xsd:integer ;
           <http://www.w3.org/2004/02/skos/core#definition> "confidence score out of 100" .


#################################################################
#    Classes
#################################################################

###  http://www.nebularis.org/ontologies/Mork#IncompleteMapping
:IncompleteMapping rdf:type owl:Class ;
                   rdfs:subClassOf :DataMapping .


###  http://www.nebularis.org/ontologies/Mork/AnonymousElement
:AnonymousElement rdf:type owl:Class ;
                  rdfs:subClassOf [ owl:intersectionOf ( :CollectionElement
                                                         [ rdf:type owl:Restriction ;
                                                           owl:onProperty :identifier ;
                                                           owl:hasValue ""
                                                         ]
                                                       ) ;
                                    rdf:type owl:Class
                                  ] ;
                  rdfs:label "anonymous entity" ;
                  <http://www.w3.org/2004/02/skos/core#definition> "Used to describe the Representation of an Entity that has no identifier, e.g., that is defined anonymously, such as an object within an array." ;
                  <http://www.w3.org/2004/02/skos/core#example> """### the Array contractingParties contains elements which provide firstName and lastName
### e.g., (JSON)
### { \"contractingParties\": [ { \"firstName\": \"Joe\", \"lastName:\", \"Blogs\" }, { \"firstName\": \"John\", \"lastName\": \"Johns\" } ] }
###

:JS_Array_ContractingParties rdf:type owl:NamedIndividual, mork:Array ;
                             mork:elementType :JS_Elem_ContractingParties ;
                             mork:identifier \"contractingParties\" ;
                             mork:path \"contract.signatories.contractingParties\" ;
                             mork:representationOf :DC_ContractingParties ;
                             mork:representationScheme :Scheme_Rep_Contracts .

:JS_Elem_ContractingParties rdf:type owl:NamedIndividual, mork:AnonymousEntity ;
                            mork:identifier \"\" ;
                            mork:memberProperty :JS_Attr_FirstName, :JS_Attr_LastName ;
                            mork:path \"contract.signatories.contractingParties[n]\" ;
                            mork:representationOf :DC_ContractingParties_Party ;
                            mork:representationScheme :Scheme_Rep_Contracts .""" .


###  http://www.nebularis.org/ontologies/Mork#Array
:Array rdf:type owl:Class ;
       rdfs:subClassOf :UnorderedCollection ;
       rdfs:label "array" ;
       rdfs:seeAlso :elementType ;
       <http://www.w3.org/2004/02/skos/core#definition> "Used to represent an Array, which is an unordered collection of elements. Elements can be associated with the array via the elementType object property." .


###  http://www.nebularis.org/ontologies/Mork#Association
:Association rdf:type owl:Class ;
             rdfs:subClassOf :Representation ;
             owl:disjointWith :Entity ;
             rdfs:label "association" ;
             <http://www.w3.org/2004/02/skos/core#definition> "Represents an association between two data Representations. This mirrors the role of Objectification in the subClass hierarchy of DataConcept." ;
             <http://www.w3.org/2004/02/skos/core#scopeNote> "By convention, mork:Association does not collect individual members, but acts as a structural component." .


###  http://www.nebularis.org/ontologies/Mork#Attribute
:Attribute rdf:type owl:Class ;
           owl:equivalentClass [ owl:intersectionOf ( [ rdf:type owl:Class ;
                                                        owl:unionOf ( [ rdf:type owl:Restriction ;
                                                                        owl:onProperty [ owl:inverseOf :memberProperty
                                                                                       ] ;
                                                                        owl:someValuesFrom :Association
                                                                      ]
                                                                      [ rdf:type owl:Restriction ;
                                                                        owl:onProperty [ owl:inverseOf :memberProperty
                                                                                       ] ;
                                                                        owl:someValuesFrom :Entity
                                                                      ]
                                                                    )
                                                      ]
                                                      [ rdf:type owl:Restriction ;
                                                        owl:onProperty :memberProperty ;
                                                        owl:qualifiedCardinality "0"^^xsd:nonNegativeInteger ;
                                                        owl:onClass :Representation
                                                      ]
                                                    ) ;
                                 rdf:type owl:Class
                               ] ;
           rdfs:subClassOf :IdentifiableElement ;
           rdfs:label "attribute (representation)" ;
           <http://www.w3.org/2004/02/skos/core#definition> "is used to denote an attribute in a representation scheme" ;
           <http://www.w3.org/2004/02/skos/core#historyNote> """Since we cannot easily capture data type constraints as data in OWL, members of this class will usually be \"shadowed\" by an owl:DataTypeProperty that is generated by a mapping process, against which the range (of possible data types) will be captured. 

The individual Attribute will then be marked as relating to the generated owl:DataTypeProperty using either the owl:sameAs axiom, or and rdfs:seeAlso annotation.""" .


###  http://www.nebularis.org/ontologies/Mork#Chaining
:Chaining rdf:type owl:Class ;
          rdfs:subClassOf :Composition ;
          owl:disjointWith :Collection .


###  http://www.nebularis.org/ontologies/Mork#Collection
:Collection rdf:type owl:Class ;
            rdfs:subClassOf :Composition ;
            rdfs:label "collection" ;
            <http://www.w3.org/2004/02/skos/core#definition> "Used to represent a collection of elements, such as a list or array." .


###  http://www.nebularis.org/ontologies/Mork#CollectionElement
:CollectionElement rdf:type owl:Class ;
                   rdfs:subClassOf :Membership ;
                   rdfs:label "collection element" ;
                   <http://www.w3.org/2004/02/skos/core#definition> "Used to describe the membership of elements within a collection." .


###  http://www.nebularis.org/ontologies/Mork#Composition
:Composition rdf:type owl:Class ;
             rdfs:subClassOf :Association ;
             rdfs:label "composition" ;
             <http://www.w3.org/2004/02/skos/core#definition> "Is used to represent a compositional association between two Representation elements. This carries the semantics that the object in a subject-predicate-object triple, should not be present in an object graph without the presence of a correponding element representing the subject." .


###  http://www.nebularis.org/ontologies/Mork#DataConcept
:DataConcept rdf:type owl:Class ;
             rdfs:subClassOf [ owl:intersectionOf ( <http://www.w3.org/2004/02/skos/core#Concept>
                                                    [ rdf:type owl:Restriction ;
                                                      owl:onProperty :conceptScheme ;
                                                      owl:someValuesFrom :TaxonomyScheme
                                                    ]
                                                  ) ;
                               rdf:type owl:Class
                             ] ;
             rdfs:label "data concept" ;
             <http://www.w3.org/2004/02/skos/core#definition> "An abstract description of a concept, representing a concept to be mapped to a representation and/or ontology scheme." ;
             <http://www.w3.org/2004/02/skos/core#scopeNote> "DataConcepts are derived from a representation scheme and mapped to an ontological scheme. An individual can be both a Representation and a DataConcept." .


###  http://www.nebularis.org/ontologies/Mork#DataMapping
:DataMapping rdf:type owl:Class ;
             rdfs:subClassOf [ owl:intersectionOf ( <http://www.w3.org/2004/02/skos/core#Concept>
                                                    [ rdf:type owl:Restriction ;
                                                      owl:onProperty :mappingScheme ;
                                                      owl:someValuesFrom :MappingScheme
                                                    ]
                                                  ) ;
                               rdf:type owl:Class
                             ] ;
             rdfs:comment "Usually a DataMapping will provide some skos:note annotation explaining the logic behind the mapping. Optionally, mapping properties may be annotated to provide additional logical explanations." ;
             rdfs:label "data mapping" ;
             <http://www.w3.org/2004/02/skos/core#definition> "is used to capture a mapping between concepts from a representation and/or concept scheme to an ontological scheme" .


###  http://www.nebularis.org/ontologies/Mork#Datum
:Datum rdf:type owl:Class ;
       rdfs:subClassOf :DataMapping ;
       rdfs:comment """The need to individuate a datum (described by a TaxonomyScheme, provided via a RepresentationScheme) in an OntologicalScheme is implied by the existence of a DataMapping, however when individuation of a DataConcept requires complex mapping steps, specificity becomes important. 

In the skos:example attached to compositeNarrowerMapping provides an example of this.""" ;
       rdfs:label "datum mapping" ;
       rdfs:seeAlso :compositeNarrowerMapping ;
       <http://www.w3.org/2004/02/skos/core#definition> "defines a mapping that explicitly states a datum must be individuated in a target OntologicalScheme" .


###  http://www.nebularis.org/ontologies/Mork#Digraph
:Digraph rdf:type owl:Class ;
         rdfs:subClassOf <http://www.w3.org/2004/02/skos/core#Concept> ,
                         [ rdf:type owl:Restriction ;
                           owl:onProperty :digraphMatch ;
                           owl:someValuesFrom :OwlAxiom
                         ] ;
         owl:deprecated "Use compositeBroaderMapping and compositeNarrowerMapping instead." .


###  http://www.nebularis.org/ontologies/Mork#Entity
:Entity rdf:type owl:Class ;
        rdfs:subClassOf :IdentifiableElement ;
        rdfs:label "entity (representation)" ;
        rdfs:seeAlso :identifier ;
        <http://www.w3.org/2004/02/skos/core#definition> "Is used to denote an entity in a representation scheme. An Entity will usually be marked with it's identify in some originating representation scheme using the identifier datatype property." .


###  http://www.nebularis.org/ontologies/Mork#IdentifiableElement
:IdentifiableElement rdf:type owl:Class ;
                     rdfs:subClassOf [ owl:intersectionOf ( :Representation
                                                            [ rdf:type owl:Restriction ;
                                                              owl:onProperty :identifier ;
                                                              owl:someValuesFrom xsd:string
                                                            ]
                                                          ) ;
                                       rdf:type owl:Class
                                     ] .


###  http://www.nebularis.org/ontologies/Mork#IndexedMapping
:IndexedMapping rdf:type owl:Class ;
                rdfs:subClassOf :DataMapping .


###  http://www.nebularis.org/ontologies/Mork/Interpolation
:Interpolation rdf:type owl:Class ;
               owl:equivalentClass [ owl:intersectionOf ( [ rdf:type owl:Restriction ;
                                                            owl:onProperty :interpolationComponent ;
                                                            owl:someValuesFrom :DataMapping
                                                          ]
                                                          [ rdf:type owl:Restriction ;
                                                            owl:onProperty :interpolationTemplate ;
                                                            owl:someValuesFrom xsd:string
                                                          ]
                                                        ) ;
                                     rdf:type owl:Class
                                   ] ;
               rdfs:subClassOf <http://www.w3.org/2004/02/skos/core#OrderedCollection> ;
               rdfs:label "interpolation template" ;
               rdfs:seeAlso :interpolationComponent ,
                            :interpolationTemplate ;
               <http://www.w3.org/2004/02/skos/core#definition> "Used to collect two or more mappings that require interpolation against a template. The syntax for referencing the mappings is simply $1, $2, $3, according to their position within the underlying OrderedCollection." ;
               <http://www.w3.org/2004/02/skos/core#example> """###  http://www.nebularis.org/ontologies/Mork#CorporateName
:ConcatCorporateName rdf:type owl:NamedIndividual , mork:Interpolation ;
               :interpolationComponent :FirstName ,
                                                            :LastName ;
               :interpolationTemplate \"$2, $1\" ,
               skos:note \"produces Lastname, Firstname, e.g., 'Vader, Darth'\".

###  http://www.nebularis.org/ontologies/Mork#FirstName
:FirstName rdf:type owl:NamedIndividual , mork:DataMapping ;
           :dataRef \"path.to.firstName\" .

###  http://www.nebularis.org/ontologies/Mork#LastName
:LastName rdf:type owl:NamedIndividual , mork:DataMapping ;
          :dataRef \"path.to.lastName\" .

###  http://www.nebularis.org/ontologies/Mork#MappingExample
:MappingExample rdf:type owl:NamedIndividual ,
                         :Datum ;
                :concatenation :ConcatCorporateName ;
                :exactRBoxMatch :corporateName .""" .


###  http://www.nebularis.org/ontologies/Mork/Lookup
:Lookup rdf:type owl:Class ;
        rdfs:subClassOf [ owl:intersectionOf ( :DataMapping
                                               [ rdf:type owl:Restriction ;
                                                 owl:onProperty :dataRef ;
                                                 owl:someValuesFrom xsd:string
                                               ]
                                             ) ;
                          rdf:type owl:Class
                        ] ;
        rdfs:label "lookup" ;
        rdfs:seeAlso :referenceDataMapping ;
        <http://www.w3.org/2004/02/skos/core#definition> "Defines a \"lookup\", from some base data to a named individual" ;
        <http://www.w3.org/2004/02/skos/core#scopeNote> """- dataRef value points to a \"path\" in the source data where the lookup (code or indicator) resides
- t-box match indicates the class to which the identified individual must belong
- r-box match indicates the relationship between the mapping subject and the identified individual (object)""" .


###  http://www.nebularis.org/ontologies/Mork#MappingScheme
:MappingScheme rdf:type owl:Class ;
               rdfs:subClassOf <http://www.w3.org/2004/02/skos/core#ConceptScheme> ;
               rdfs:label "mapping scheme" ;
               <http://www.w3.org/2004/02/skos/core#definition> "a scheme that captures mappings between concepts, from a RepresentationScheme to an OntologicalScheme" .


###  http://www.nebularis.org/ontologies/Mork#Membership
:Membership rdf:type owl:Class ;
            rdfs:subClassOf :Representation ;
            rdfs:label "membership" ;
            <http://www.w3.org/2004/02/skos/core#definition> "Conceptual representation of the notion of \"membership\" within some containing Representation element." ;
            <http://www.w3.org/2004/02/skos/core#scopeNote> "By convention, individuals should not made direct members of this class, but rather belong to its subclasses." .


###  http://www.nebularis.org/ontologies/Mork#Objectification
:Objectification rdf:type owl:Class ;
                 owl:equivalentClass [ owl:intersectionOf ( [ rdf:type owl:Restriction ;
                                                              owl:onProperty :broadConceptRole ;
                                                              owl:minQualifiedCardinality "1"^^xsd:nonNegativeInteger ;
                                                              owl:onClass <http://www.w3.org/2004/02/skos/core#Concept>
                                                            ]
                                                            [ rdf:type owl:Restriction ;
                                                              owl:onProperty :narrowConceptRole ;
                                                              owl:minQualifiedCardinality "1"^^xsd:nonNegativeInteger ;
                                                              owl:onClass <http://www.w3.org/2004/02/skos/core#Concept>
                                                            ]
                                                          ) ;
                                       rdf:type owl:Class
                                     ] ;
                 rdfs:subClassOf :DataConcept ;
                 <http://www.w3.org/2004/02/skos/core#altLabel> "RoleAssociation" ;
                 <http://www.w3.org/2004/02/skos/core#definition> "Represents an \"objectified fact\" relating two DataConcepts to one another with a specific set of roles in mind." ;
                 <http://www.w3.org/2004/02/skos/core#editorialNote> """An Objectification allows instances of relationships to be treated as entities in their own right, sometimes referred to as “reification” (e.g., in UML, mediated mediated by association classes), “objectification”, or “nesting”, e.g., in Object-Role Modeling (ORM) notation.

Objectification is related to the linguistic activity of nominalization. In the context of Mork, an Objectification plays a similar role to an association class (in UML), insomuch as RDF does not allow us to attribute facts (i.e., properties) to the edges between nodes in the graph, therefore an intermediate node serves to allow us to capture the notion of \"relatedness\" in such a way that it can be mapped.

See Terry Halpin's paper on objectified facts for more details: https://www.orm.net/pdf/objectification.pdf""" ;
                 <http://www.w3.org/2004/02/skos/core#example> """### Consider the following Objectification and associated mapping.
### The closeMatch on 'contract:signatory' points to an objectProperty 
### in the target ontology, with annotations on the property providing context
### to the mapping recommendation

:Concept_Conditions_CombinedLimitSymbols 
                 rdf:type owl:NamedIndividual,
                 mork:Objectification ; 
           mork:broadConceptRole :Rep_Conditions ;
           mork:conceptScheme :Taxa_Scheme ; 
           mork:narrowConceptRole :Rep_CombinedLimitSymbols ;
           skos:note \"Models an association between Rep_Conditions and the attribute combinedLimitSymbols, which is represented by Rep_CombinedLimitSymbols\" .

:Mapping_Signatories 
                 rdf:type owl:NamedIndividual, mork:DataMapping ;
           skos:closeMatch contract:signatory ;
           mork:mappingScheme :Scheme_Map_Contracts ;
           mork:weighting 80 ;
           skos:note \"signatories may be related to the ontological concept signatory\" .

[ rdf:type owl:Axiom ;
   owl:annotatedSource :Mapping_Signatories ;
   owl:annotatedProperty skos:closeMatch ;
   owl:annotatedTarget contract:signatory ;
   skos:note \"close match on 'signatories' and owl:objectProperty 'signatory'\"
 ] .""" .


###  http://www.nebularis.org/ontologies/Mork#OntologicalScheme
:OntologicalScheme rdf:type owl:Class ;
                   rdfs:subClassOf <http://www.w3.org/2004/02/skos/core#ConceptScheme> ;
                   rdfs:label "ontological scheme" .


###  http://www.nebularis.org/ontologies/Mork#OrderedCollection
:OrderedCollection rdf:type owl:Class ;
                   owl:equivalentClass [ rdf:type owl:Restriction ;
                                         owl:onProperty :orderedItems ;
                                         owl:hasValue "true"^^xsd:boolean
                                       ] ;
                   rdfs:subClassOf :Collection .


###  http://www.nebularis.org/ontologies/Mork#OwlAxiom
:OwlAxiom rdf:type owl:Class ;
          owl:equivalentClass [ owl:intersectionOf ( <http://www.w3.org/2004/02/skos/core#Concept>
                                                     [ rdf:type owl:Restriction ;
                                                       owl:onProperty <http://www.w3.org/2004/02/skos/core#inScheme> ;
                                                       owl:someValuesFrom :OntologicalScheme
                                                     ]
                                                   ) ;
                                rdf:type owl:Class
                              ] ;
          rdfs:comment """For processing environments where objectProperties cannot refer to an arbitrary owl:Thing is not possible, each axiom in the OntologicalScheme will be connected to an assertion of this type via the owl:sameAs mechanism.

Can also be used to instantiate individual members of this class that represent owl:Nothing (which is a problematic assertion in most processing environments).

It is recommended that each member of this class also uses the rdfs:seeAlso annotation to record the owl:Thing is points to, for environments that do not properly support the owl:sameAs axiom.""" ;
          rdfs:label "owl axiom" ;
          <http://www.w3.org/2004/02/skos/core#definition> "used to denote an axiom in an OWL ontology" ;
          <http://www.w3.org/2004/02/skos/core#example> """###  Mapping between the concept Signatory_acceptingParty and an objectProperty 
###  in the target ontology (acceptingParty), met via Onto_Assoc_Contract_acceptingParty
###  since placing an instance of owl:ObjectProperty in the object position of an RDF 
###  triple is disallowed by some processing environments (e.g., owlapi).
###
###  Note that we mark Onto_Assoc_Contract_acceptingParty as representing acceptingParty
###  via the owl:sameAs construct.
###

:Map_Signatory_acceptingParty rdf:type owl:NamedIndividual ;
              skos:relatedMatch Onto_Assoc_Contract_acceptingParty ;
              mork:hypothesisMapping :Map_Signatory_Party ;
              mork:mappingScheme :Scheme_Map_Contracts .

:Onto_Assoc_Contract_acceptingParty 
                       rdf:type owl:NamedIndividual, 
                       mork:OwlObjectProperty ;
              owl:sameAs <http://www.nebularis.org/hyperthunk/examples/Contract#acceptingParty> ;
              mork:conceptName \"acceptingParty\" ;
              mork:iri \"http://www.nebularis.org/hyperthunk/examples/Contract/acceptingParty\" ;
              mork:ontologicalScheme :Scheme_Onto_Contracts .""" ;
          <http://www.w3.org/2004/02/skos/core#scopeNote> """The OwlAxiom members of an OntologicalScheme are not interrelated using skos notation, since that information is already present in the ontology itself.

Rather, the behaviour when mapping data into (and out of) an OntologicalScheme is captured by each DataMapping such that ?mappping skos:inScheme :MappingScheme""" .


###  http://www.nebularis.org/ontologies/Mork#OwlClass
:OwlClass rdf:type owl:Class ;
          rdfs:subClassOf :OwlAxiom ;
          rdfs:label "owl class" ;
          <http://www.w3.org/2004/02/skos/core#definition> "Represents an OWL Class." .


###  http://www.nebularis.org/ontologies/Mork#OwlDataProperty
:OwlDataProperty rdf:type owl:Class ;
                 rdfs:subClassOf :OwlAxiom ;
                 rdfs:label "owl data property" ;
                 <http://www.w3.org/2004/02/skos/core#definition> "Represents an OWL DataProperty" .


###  http://www.nebularis.org/ontologies/Mork#OwlObjectProperty
:OwlObjectProperty rdf:type owl:Class ;
                   rdfs:subClassOf :OwlAxiom ;
                   rdfs:label "owl object property" ;
                   <http://www.w3.org/2004/02/skos/core#definition> "Represents an OWL ObjectProperty" .


###  http://www.nebularis.org/ontologies/Mork#Referencing
:Referencing rdf:type owl:Class ;
             rdfs:subClassOf :Association .


###  http://www.nebularis.org/ontologies/Mork#Representation
:Representation rdf:type owl:Class ;
                rdfs:subClassOf <http://www.w3.org/2004/02/skos/core#Concept> ,
                                [ rdf:type owl:Restriction ;
                                  owl:onProperty <http://www.w3.org/2004/02/skos/core#inScheme> ;
                                  owl:someValuesFrom :RepresentationScheme
                                ] ;
                rdfs:label "representation" ;
                <http://www.w3.org/2004/02/skos/core#definition> "Is used to describe the representation of a DataConcept. Some individuals may be both DataConcept and Representation." .


###  http://www.nebularis.org/ontologies/Mork#RepresentationScheme
:RepresentationScheme rdf:type owl:Class ;
                      rdfs:subClassOf [ owl:intersectionOf ( <http://www.w3.org/2004/02/skos/core#ConceptScheme>
                                                             [ rdf:type owl:Restriction ;
                                                               owl:onProperty :format ;
                                                               owl:someValuesFrom :SerializationFormat
                                                             ]
                                                           ) ;
                                        rdf:type owl:Class
                                      ] ;
                      rdfs:label "representation scheme" ;
                      <http://www.w3.org/2004/02/skos/core#definition> "a scheme that maps concepts to their representation" .


###  http://www.nebularis.org/ontologies/Mork#ScalarValueElement
:ScalarValueElement rdf:type owl:Class ;
                    rdfs:subClassOf :AnonymousElement ;
                    rdfs:label "scalar value" ;
                    <http://www.w3.org/2004/02/skos/core#altLabel> "scalar collection element value" ;
                    <http://www.w3.org/2004/02/skos/core#definition> "Used to describe scalar (atomic) values as members of a collection, such as an Array." ;
                    <http://www.w3.org/2004/02/skos/core#example> """###  http://www.nebularis.org/hyperthunk/Mapping#Rep_CombinedLimitSymbols
:Rep_CombinedLimitSymbols rdf:type owl:NamedIndividual , 
                                    mork:Array ;
                          mork:elementType :Rep_CombinedLimitSymbols_Element2147483650 ;
                          mork:representationOf :Rep_CombinedLimitSymbols ;
                          mork:representationScheme :Mapping_Representation ;
                          mork:identifier \"combinedLimitSymbols\" ;
                          mork:orderedItems \"false\"^^xsd:boolean .

###  http://www.nebularis.org/hyperthunk/Mapping#Rep_CombinedLimitSymbols_Element2147483650
:Rep_CombinedLimitSymbols_Element2147483650 rdf:type owl:NamedIndividual , 
                                    mork:ScalarValueElement> ;
                          mork:representationScheme :Mapping_Representation ;
                          mork:identifier \"combinedLimitSymbols_Element2147483650\" ;
                          rdfs:seeAlso :combinedLimitSymbols_Element2147483650 .""" .

[ rdf:type owl:Axiom ;
   owl:annotatedSource :ScalarValueElement ;
   owl:annotatedProperty <http://www.w3.org/2004/02/skos/core#example> ;
   owl:annotatedTarget """###  http://www.nebularis.org/hyperthunk/Mapping#Rep_CombinedLimitSymbols
:Rep_CombinedLimitSymbols rdf:type owl:NamedIndividual , 
                                    mork:Array ;
                          mork:elementType :Rep_CombinedLimitSymbols_Element2147483650 ;
                          mork:representationOf :Rep_CombinedLimitSymbols ;
                          mork:representationScheme :Mapping_Representation ;
                          mork:identifier \"combinedLimitSymbols\" ;
                          mork:orderedItems \"false\"^^xsd:boolean .

###  http://www.nebularis.org/hyperthunk/Mapping#Rep_CombinedLimitSymbols_Element2147483650
:Rep_CombinedLimitSymbols_Element2147483650 rdf:type owl:NamedIndividual , 
                                    mork:ScalarValueElement> ;
                          mork:representationScheme :Mapping_Representation ;
                          mork:identifier \"combinedLimitSymbols_Element2147483650\" ;
                          rdfs:seeAlso :combinedLimitSymbols_Element2147483650 .""" ;
   rdfs:comment _:genid86
 ] .

_:genid86 rdfs:comment "Shows an Array and its corresponding element type" .


###  http://www.nebularis.org/ontologies/Mork#SerializationFormat
:SerializationFormat rdf:type owl:Class .


###  http://www.nebularis.org/ontologies/Mork#SetListing
:SetListing rdf:type owl:Class ;
            owl:equivalentClass [ rdf:type owl:Restriction ;
                                  owl:onProperty :uniqueItems ;
                                  owl:hasValue "true"^^xsd:boolean
                                ] ;
            rdfs:subClassOf :Collection .


###  http://www.nebularis.org/ontologies/Mork#TaxonomyScheme
:TaxonomyScheme rdf:type owl:Class ;
                rdfs:subClassOf <http://www.w3.org/2004/02/skos/core#ConceptScheme> .


###  http://www.nebularis.org/ontologies/Mork#UnorderedCollection
:UnorderedCollection rdf:type owl:Class ;
                     owl:equivalentClass [ rdf:type owl:Restriction ;
                                           owl:onProperty :orderedItems ;
                                           owl:hasValue "false"^^xsd:boolean
                                         ] ;
                     rdfs:subClassOf :Collection .


###  http://www.nebularis.org/ontologies/Mork#WeightedMatch
:WeightedMatch rdf:type owl:Class ;
               rdfs:subClassOf :DataMapping ,
                               [ rdf:type owl:Restriction ;
                                 owl:onProperty :weighting ;
                                 owl:someValuesFrom xsd:integer
                               ] ;
               rdfs:label "weighted match" ;
               <http://www.w3.org/2004/02/skos/core#definition> "is used to score a potential match (between concept taxa and ontological facts)" ;
               <http://www.w3.org/2004/02/skos/core#scopeNote> "each member of this class may carry skos:note and rdfs:seeAlso that explain the rules used to arrive at the match" .


###  http://www.w3.org/1999/02/22-rdf-syntax-ns#List
rdf:List rdf:type owl:Class .


###  http://www.w3.org/2004/02/skos/core#Concept
<http://www.w3.org/2004/02/skos/core#Concept> owl:equivalentClass [ rdf:type owl:Restriction ;
                                                                    owl:onProperty <http://www.w3.org/2004/02/skos/core#mappingRelation> ;
                                                                    owl:someValuesFrom <http://www.w3.org/2004/02/skos/core#Concept>
                                                                  ] .


#################################################################
#    Individuals
#################################################################

###  http://www.nebularis.org/ontologies/Mork#Bottom
:Bottom rdf:type owl:NamedIndividual ,
                 :OwlAxiom ;
        owl:sameAs :OwlNothing .


###  http://www.nebularis.org/ontologies/Mork#OwlNothing

###  http://www.nebularis.org/ontologies/Mork/DataExample
:DataExample rdf:type owl:NamedIndividual ,
                      :Datum ;
             :mappingScheme :Scheme ;
             :dataRef "path.to.value" .


###  http://www.nebularis.org/ontologies/Mork/JSON
:JSON rdf:type owl:NamedIndividual ,
               :SerializationFormat ;
      rdfs:isDefinedBy "https://datatracker.ietf.org/doc/html/rfc7159.html" .


###  http://www.nebularis.org/ontologies/Mork#OwlNothing
:OwlNothing rdf:type owl:NamedIndividual ,
                     :OwlAxiom .


###  http://www.nebularis.org/ontologies/Mork/Scheme
:Scheme rdf:type owl:NamedIndividual ,
                 :MappingScheme .


###  http://www.nebularis.org/ontologies/Mork/XML
:XML rdf:type owl:NamedIndividual ,
              :SerializationFormat ;
     rdfs:isDefinedBy "https://www.w3.org/TR/xml/" .


###  http://www.nebularis.org/ontologies/Mork#YAML
:YAML rdf:type owl:NamedIndividual ,
               :SerializationFormat ;
      rdfs:isDefinedBy "https://yaml.org/spec/" .


[ rdfs:comment "Shows an array and its corresponding scalar/atomic element type"
] .

#################################################################
#    General axioms
#################################################################

[ rdf:type owl:AllDisjointClasses ;
   owl:members ( :OrderedCollection
                 :SetListing
                 :UnorderedCollection
               )
 ] .


[ rdf:type owl:AllDisjointProperties ;
  owl:members ( :broaderMapping
                :closeMapping
                :deferredMapping
                :hypothesisMapping
                :narrowerMapping
              )
] .


###  Generated by the OWL API (version 4.5.29.2024-05-13T12:11:03Z) https://github.com/owlcs/owlapi
